Prove properties about interface(s) (schemes)

Runtime/Interface.lean
@@ -14,6 +14,10 @@ abbrev Scheme.restrict (σ : Scheme) (Sub : Type) [DecidableEq Sub] [InjectiveCo
   vars := Sub
   type var := σ.type var
 
+@[simp]
+theorem Scheme.restrict_type (σ : Scheme) (Sub : Type) [DecidableEq Sub] [InjectiveCoe Sub σ.vars] (var : Sub) : 
+  (σ.restrict Sub).type var = σ.type var := rfl
+
 abbrev Scheme.union (σ₁ σ₂ : Scheme) : Scheme where
   vars := Sum σ₁.vars σ₂.vars
   type
@@ -22,30 +26,49 @@ abbrev Scheme.union (σ₁ σ₂ : Scheme) : Scheme where
 
 infix:65 " ⊎ " => Scheme.union
 
-abbrev Scheme.bUnion {Schemes : Type} [DecidableEq Schemes] (σ : Schemes → Scheme) : Scheme where
-  vars := Σ scheme : Schemes, (σ scheme).vars
-  type := fun ⟨scheme, var⟩ => (σ scheme).type var
+@[simp]
+theorem Scheme.union_type_left (σ₁ σ₂ : Scheme) (var : σ₁.vars) : 
+  (σ₁ ⊎ σ₂).type (.inl var) = σ₁.type var := rfl
+
+@[simp]
+theorem Scheme.union_type_right (σ₁ σ₂ : Scheme) (var : σ₂.vars) : 
+  (σ₁ ⊎ σ₂).type (.inr var) = σ₂.type var := rfl
+
+-- σs is an I-indexed family of schemes.
+abbrev Scheme.bUnion (σs : I → Scheme) [DecidableEq I] : Scheme where
+  vars := (i : I) × (σs i).vars
+  type := fun ⟨i, var⟩ => (σs i).type var
 
 prefix:100 " ⨄ " => Scheme.bUnion
 
-@[reducible]
-instance {σ : Scheme} {Sub : Type} [DecidableEq Sub] [InjectiveCoe Sub σ.vars] : InjectiveCoe (σ.restrict Sub).vars σ.vars := 
-  inferInstance
-
-theorem Scheme.restrict_preserves_type (σ : Scheme) (Sub : Type) [DecidableEq Sub] [InjectiveCoe Sub σ.vars] (var : Sub) : 
-  (σ.restrict Sub).type var = σ.type var := rfl
-
-abbrev _root_.Interface (σ : Interface.Scheme) := (var : σ.vars) → (σ.type var)
+@[simp]
+theorem Scheme.bUnion_type (σs : I → Scheme) [DecidableEq I] (var : (σs i).vars) : 
+  (⨄ σs).type ⟨i, var⟩ = (σs i).type var := rfl
 
 end Interface
+
+abbrev Interface (σ : Interface.Scheme) := (var : σ.vars) → (σ.type var)
 
 abbrev Interface? (σ : Interface.Scheme) := (var : σ.vars) → Option (σ.type var)
 
 def Interface?.empty : Interface? σ := fun _ => none
 
+@[simp]
+theorem Interface?.empty_none : Interface?.empty var = none := rfl
+
 def Interface?.isPresent (i : Interface? σ) (var : σ.vars) : Bool :=
   i var |>.isSome
+
+@[simp]
+theorem Interface?.isPresent_def (i : Interface? σ) : i.isPresent var ↔ ∃ v, i var = some v := by
+  simp [isPresent, Option.isSome_def]
 
 -- Merge i₂ into i₁.
 def Interface?.merge (i₁ i₂ : Interface? σ) : Interface? σ :=
   fun var => i₂ var |>.orElse fun _ => i₁ var
+
+theorem Interface?.merge_val₁ (i₁ i₂ : Interface? σ) : (i₂ var = none) → (i₁.merge i₂) var = i₁ var := by
+  simp_all [merge, Option.orElse]
+
+theorem Interface?.merge_val₂ (i₁ i₂ : Interface? σ) : (i₂ var = some v) → (i₁.merge i₂) var = some v := by
+  simp_all [merge, Option.orElse]
